lean_project/AbsSat.lean
@@ -36,4 +36,5 @@ import AbsSat.GraphPath.Model.Up
 import AbsSat.GraphPath.Model.L6Up
 import AbsSat.GraphPath.Model.Review
 import AbsSat.GraphPath.Model.CleanInvalid
+import AbsSat.GraphPath.Model.Coherence
 import AbsSat.GraphPath.Model.L6Search
